simplify some proofs

src/K/tableau.lean
@@ -1,21 +1,22 @@
 import .full_language .jump
 
-def classical_is_sat (Γ : list fml) : bool :=
+def fml_is_sat (Γ : list fml) : bool :=
 match tableau (list.map fml.to_nnf Γ) with
 | node.closed _ _ _ := ff
 | node.open_ _ := tt
 end
 
-theorem classical_correctness (Γ : list fml) : classical_is_sat Γ = tt ↔ ∃ (st : Type) (k : kripke st) s, fml_sat k s Γ := 
+theorem classical_correctness (Γ : list fml) : 
+fml_is_sat Γ = tt ↔ ∃ (st : Type) (k : kripke st) s, fml_sat k s Γ := 
 begin
-  cases h : classical_is_sat Γ,
+  cases h : fml_is_sat Γ,
   constructor,
   { intro, contradiction },
   { intro hsat, cases eq : tableau (list.map fml.to_nnf Γ), 
     rcases hsat with ⟨w, k, s, hsat⟩,
     apply false.elim, apply a, rw trans_sat_iff at hsat, exact hsat,
-    { dsimp [classical_is_sat] at h, rw eq at h, contradiction } },
-  { split, intro, dsimp [classical_is_sat] at h, 
+    { dsimp [fml_is_sat] at h, rw eq at h, contradiction } },
+  { split, intro, dsimp [fml_is_sat] at h, 
      cases eq : tableau (list.map fml.to_nnf Γ),
      { rw eq at h, contradiction },
   { split, split, split, have := a_1.2, rw ←trans_sat_iff at this, 
@@ -30,6 +31,6 @@ def fml.exm : fml := or (var 1) (neg (var 1))
 
 def K : fml := impl (box (impl (var 1) (var 2))) (impl (box $ var 1) (box $ var 2))
 
-#eval classical_is_sat [neg fml.exm]
+#eval fml_is_sat [neg fml.exm]
 
-#eval classical_is_sat [neg K]
+#eval fml_is_sat [neg K]
